coq/JsInit.v
@@ -289,14 +289,20 @@ Definition object_prealloc_function_proto :=
   let P := Heap.write P "length" (attrib_constant 0) in (* todo: can we use write_constant? *)
   (* let P := write_native P "toString" prealloc_function_proto_to_string in *) (* LATER *)
   (* let P := write_native P "apply" prealloc_function_proto_apply in *) (* LATER *)
-  (* let P := write_native P "call" prealloc_function_proto_call in *) (* LATER *)
-  (* let P := write_native P "bind" prealloc_function_proto_bind in *) (* LATER *)
+  let P := write_native P "call" prealloc_function_proto_call in 
+  let P := write_native P "bind" prealloc_function_proto_bind in 
   (* LATER: complete list *)
 
   (* LATER: why this construct here and not the usual (see other builtins), i.e. just 
      [object_create_builtin prealloc_object_proto "Function" P]? *)
   let O := object_create_builtin prealloc_object_proto "Function" P in
   object_with_invokation O None (Some (call_prealloc prealloc_function_proto)) None.
+
+Definition function_proto_call_function_object :=
+  object_create_prealloc_call prealloc_function_proto_call 1 Heap.empty.
+  
+Definition function_proto_bind_function_object :=
+  object_create_prealloc_call prealloc_function_proto_bind 1 Heap.empty.
 
 (**************************************************************)
 (** Number object *)
@@ -348,7 +354,8 @@ Definition number_proto_value_of_function_object :=
 Definition object_prealloc_array :=
   let P := Heap.empty in
   let P := write_constant P "prototype" prealloc_array_proto in
-  let P := write_constant P "length" 1 in (* LATER:  Implement the full specification given in the paragraph starting Section 15.4 instead of his dummy object. *)
+  let P := write_constant P "length" 1 in 
+  (* LATER:  Implement the full specification given in the paragraph starting Section 15.4 instead of his dummy object. *)
   (* LATER *)
   object_create_prealloc_constructor prealloc_array 1 P.
 
@@ -554,6 +561,10 @@ Definition object_heap_initial_function_objects_3 (h : Heap.heap object_loc obje
   let h := Heap.write h prealloc_object_proto_has_own_prop object_proto_has_own_prop_function_object in
   let h := Heap.write h prealloc_object_proto_is_prototype_of object_proto_is_prototype_of_function_object in
   let h := Heap.write h prealloc_object_proto_prop_is_enumerable object_proto_prop_is_enumerable_function_object in
+
+  (* Function objects of Function.prototype *)
+  let h := Heap.write h prealloc_function_proto_call function_proto_call_function_object in
+  let h := Heap.write h prealloc_function_proto_bind function_proto_bind_function_object in
 
   (* Function objects of Array.prototype *)
   let h := Heap.write h prealloc_array_proto_pop array_proto_pop_function_object in
